syntactic sugar

src/Example.Check.Simple.fst
@@ -3,12 +3,12 @@ module Example.Check.Simple
 
 module Exp = Pipit.Exp.Base
 
-// open Pipit.System.Base
-// open Pipit.System.Ind
-// open Pipit.System.Exp
+open Pipit.System.Base
+open Pipit.System.Ind
+open Pipit.System.Exp
 
 module T = FStar.Tactics
-module Sugar = Pipit.SugarX3
+module Sugar = Pipit.SugarX4
 open Sugar
 
 let tac_nbe (): T.Tac unit = T.norm [primops; iota; delta; zeta; nbe]
@@ -20,12 +20,12 @@ let tac_nbe (): T.Tac unit = T.norm [primops; iota; delta; zeta; nbe]
        (if p then 1 else 0)
 *)
 inline_for_extraction
-let count_when (p: stream bool): Stream (stream int) =
+let count_when (p: s bool): s int =
  rec' (fun count ->
    fby 0 count +^ (ite p z1 z0))
 
 (* forall e. count_when false <= count_when e <= count_when true *)
-let count_when_prop (e: stream bool): Stream (stream unit) =
+let count_when_prop (e: s bool): s unit =
   let' (count_when ff) (fun count_when_false ->
   let' (count_when e) (fun count_when_e ->
   let' (count_when tt) (fun count_when_true ->
@@ -33,14 +33,38 @@ let count_when_prop (e: stream bool): Stream (stream unit) =
   check' "cwe<=cwt" (count_when_e <=^ count_when_true) (
   pure ())))))
 
-let run (e: unit -> Stream 'a) : 'a =
-  let (a, _) = reify (e ()) { fresh = 0 } in
+let run (e: s 'a) : Exp.exp [] 'a =
+  let (a, _) = e { fresh = 0 } in
   a
 
+let count (): s int =
+  rec' (fun count -> fby 0 count +^ z1)
 
-let sdf (): Stream unit =
-  let xe = run (fun _ -> count_when_prop tt) in
-  assert (xe == (pure ())) by (T.norm [primops; iota; delta]; T.norm [nbe]; T.dump "")
+let count_when__0_prop (e: s bool): s unit =
+  check' "0 <= count_when e" (z0 <=^ z1) (pure ())
+
+
+let sys =
+  system_of_exp (run (count_when__0_prop ff))
+
+#push-options "--print_full_names --print_bound_var_types"
+let prove (fv: sem_freevars): Lemma (ensures base_case (sys fv)) =
+  assert (base_case (sys fv)) by (T.norm [primops; iota; delta; zeta; nbe]; T.dump "")
+  // assert (base_case (sys fv)) by (tac_nbe (); T.dump "")
+
+
+
+let doit (): unit =
+  let xe = run (count_when_prop (fresh bool)) in
+
+  assert (xe == Exp.XVal ()) by (T.norm [primops; iota; delta; zeta; nbe]; T.norm [delta_fully ["Pipit.SugarX3.STREAM?.reflect"]]; T.dump "")
+  // by (tac_nbe (); T.dump "")
+
+
+let sdf (): unit =
+  let xe = run (fun () -> 1) in
+  let xy = run (fun () -> 1) in
+  assert (xe == xy) by (T.norm [primops; iota; delta; nbe]; T.dump "")
   // by (tac_nbe (); T.dump "")
 
 
