src/Pipit.System.Base.fst
@@ -3,6 +3,10 @@ module Pipit.System.Base
 
 module C = Pipit.Context
 
+type xprop = bool
+
+type checks (state: Type) = list (string & (state -> prop))
+
 (* Step functions are relations so that we can express non-deterministic systems.
    The recursive dependency for recursive binders XMu is easier to express as a
    relation too. The result type is `prop`, rather than a computational boolean,
@@ -21,102 +25,122 @@ type system (input: Type) (state: Type) (result: Type) = {
     (* Return value *)
     r: result ->
     prop;
+
+  (* Properties to check *)
+  chck: checks state;
 }
 
+(* A system with "oracles", which let us draw out the quantifiers to the top level *)
+// let osystem (input: Type) (oracle: Type) (state: Type) (result: Type) = system (input & oracle) state result
+
+let map_checks (#state #state': Type) (f: state' -> state) (chck: checks state): checks state' =
+  List.Tot.map (fun (name, x) -> (name, (fun s -> x (f s)))) chck
+
+(* Manual instance for universes *)
+let app_checks (#state: Type) (chck1 chck2: checks state): checks state =
+  List.Tot.append chck1 chck2
+
+
 let rec system_stepn
-  (#outer: nat)
   (#input #state #result: Type)
   (t: system input state result)
-  (inputs: C.vector input outer)
-  (vs: C.vector result outer)
+  (inputs: list (input & result))
   (s': state): prop =
-  match inputs, vs with
-  | [], [] -> t.init s'
-  | (row :: inputs'), r :: vs' ->
+  match inputs with
+  | [] -> t.init s'
+  | ((row, r) :: inputs') ->
     exists (s0: state).
-    system_stepn #(outer - 1) t inputs' vs' s0 /\
+    system_stepn t inputs' s0 /\
     t.step row s0 s' r
 
 let system_input (#input: Type): system input unit input =
   { init = (fun s -> True);
-    step = (fun i s s' r -> r == i) }
+    step = (fun i s s' r -> r == i);
+    chck = [];
+  }
 
 let system_const (#input #result: Type) (v: result): system input unit result =
   { init = (fun s -> True);
-    step = (fun i s s' r -> r == v) }
+    step = (fun i s s' r -> r == v);
+    chck = [];
+  }
+
+// why is this necessary? issue with type inference for prop vs logical
+let prop_holds (p: prop): prop = p
+
+let system_check (#input #state: Type) (name: string)
+  (t1: system input state xprop):
+       system input (xprop & state) xprop =
+  { init = (fun (chck, s) -> chck = true /\ t1.init s);
+    step = (fun i (_, s) (chck', s') r ->
+        t1.step i s s' r /\
+        r = chck');
+    chck = (name, (fun (chck, s) -> chck == true)) :: map_checks snd t1.chck;
+  }
+
+let system_ap2 (#input #state1 #state2 #value1 #value2: Type)
+  (t1: system input state1 (value1 -> value2))
+  (t2: system input state2 value1):
+       system input (state1 & state2) value2 =
+  {
+    init = (fun (s1, s2) -> t1.init s1 /\ t2.init s2);
+    step = (fun i (s1, s2) (s1', s2') r ->
+      exists (f: value1 -> value2) (a: value1).
+        t1.step i s1 s1' f /\
+        t2.step i s2 s2' a /\
+        r == f a);
+    chck =
+      app_checks (map_checks fst t1.chck) (map_checks snd t2.chck);
+  }
+
 
 let system_map (#input #state1 #value1 #result: Type) (f: value1 -> result)
   (t1: system input state1 value1):
        system input state1 result =
   { init = t1.init;
     step = (fun i s s' r ->
-     let s1  = s in
-     let s1' = s' in
-     exists (r1: value1).
-       t1.step i s1 s1' r1 /\
-       r == f r1)
+      exists (r1: value1).
+       t1.step i s s' r1 /\
+       r == f r1);
+    chck = t1.chck;
   }
 
-let rec system_map_sem (#outer: nat) (#input #state1 #value1 #result: Type) (f: value1 -> result)
+let rec system_map_sem (#input #state1 #value1 #result: Type) (f: value1 -> result)
   (t1: system input state1 value1)
-  (inputs: C.vector input outer)
-  (vs: C.vector value1 outer)
+  (inputs: list (input & value1))
   (s': state1):
-    Lemma (requires system_stepn t1 inputs vs s')
-      (ensures system_stepn (system_map f t1) inputs (C.vector_map f vs) s') =
- match inputs, vs with
- | [], [] -> ()
- | i :: is', v :: vs' ->
-   eliminate exists (s0: state1). system_stepn #(outer - 1) t1 is' vs' s0 /\ t1.step i s0 s' v
-   returns system_stepn (system_map f t1) inputs (C.vector_map f vs) s'
+    Lemma (requires system_stepn t1 inputs s')
+      (ensures system_stepn (system_map f t1) (List.Tot.map (fun (i,v) -> (i, f v)) inputs) s') =
+ match inputs with
+ | []  -> ()
+ | (i, v) :: is' ->
+   eliminate exists (s0: state1). system_stepn t1 is' s0 /\ t1.step i s0 s' v
+   returns system_stepn (system_map f t1) (List.Tot.map (fun (i,v) -> (i, f v)) inputs) s'
    with hEx.
-        system_map_sem #(outer - 1) f t1 is' vs' s0
-
-let system_map2 (#input #state1 #state2 #value1 #value2 #result: Type) (f: value1 -> value2 -> result)
-  (t1: system input state1 value1)
-  (t2: system input state2 value2):
-       system input (state1 * state2) result =
-  {
-    init = (fun (s1, s2) -> t1.init s1 /\ t2.init s2);
-    step = (fun i (s1, s2) (s1', s2') r ->
-     exists (r1: value1) (r2: value2).
-               t1.step i s1 s1' r1 /\
-               t2.step i s2 s2' r2 /\
-               r == f r1 r2)
-  }
-
-let system_ite (#input #statep #state1 #state2 #valuep #result: Type) (f: valuep -> bool)
-  (tp: system input statep valuep)
-  (t1: system input state1 result)
-  (t2: system input state2 result):
-       system input (statep * state1 * state2) result =
-  {
-    init = (fun (sp, s1, s2) -> tp.init sp /\ t1.init s1 /\ t2.init s2);
-    step = (fun i (sp, s1, s2) (sp', s1', s2') r ->
-     exists (rp: valuep) (r1: result) (r2: result).
-               tp.step i sp sp' rp /\
-               t1.step i s1 s1' r1 /\
-               t2.step i s2 s2' r2 /\
-               r == (if f rp then r1 else r2))
-  }
+        system_map_sem f t1 is' s0
 
 let system_pre (#input #state1 #v: Type) (init: v)
   (t1: system input state1 v):
-       system input (state1 * v) v =
+       system input (state1 & v) v =
   { init = (fun (s1, v) -> t1.init s1 /\ v == init);
     step = (fun i (s1, v) (s1', v') r ->
-      t1.step i s1 s1' v' /\ r == v)
+      t1.step i s1 s1' v' /\ r == v);
+    chck = map_checks fst t1.chck;
   }
 
 let system_then (#input #state1 #state2 #v: Type)
   (t1: system input state1 v)
   (t2: system input state2 v):
-       system input (bool * state2) v =
-  { init = (fun (init,s2) -> init = true /\ t2.init s2);
-    step = (fun i (init, s2) (init', s2') r ->
+       system input (bool & state1 & state2) v =
+  { init = (fun (init,s1,s2) -> init = true /\ t1.init s1 /\ t2.init s2);
+    step = (fun i (init,s1,s2) (init',s1',s2') r ->
      if init
-     then exists s1 s1' r'. t1.init s1 /\ t1.step i s1 s1' r /\ t2.step i s2 s2' r' /\ init' = false
-     else init' = false /\ t2.step i s2 s2' r)
+     then exists r'. t1.init s1 /\ t1.step i s1 s1' r /\ t2.step i s2 s2' r' /\ init' = false
+     else init' = false /\ t2.step i s2 s2' r);
+    chck = app_checks
+      // Maybe we could relax this to something like "i ==> s1'" as the check for t1 only needs to hold on the first step...
+      (map_checks (fun (i,s1,s2) -> s1) t1.chck)
+      (map_checks (fun (i,s1,s2) -> s2) t2.chck);
   }
 
 let system_mu (#input #input' #state1 #v: Type)
@@ -124,17 +148,38 @@ let system_mu (#input #input' #state1 #v: Type)
   (t1: system input' state1 v):
        system input state1 v =
   { init = t1.init;
-    step = (fun i s s' r -> t1.step (extend i r) s s' r)
+    step = (fun i s s' r -> t1.step (extend i r) s s' r);
+    chck = t1.chck;
   }
 
 let system_let (#input #input' #state1 #state2 #v1 #v2: Type)
   (extend: input -> v1 -> input')
   (t1: system input  state1 v1)
   (t2: system input' state2 v2):
-       system input (state1 * state2) v2 =
+       system input (state1 & state2) v2 =
   { init = (fun (s1, s2) -> t1.init s1 /\ t2.init s2);
     step = (fun i (s1, s2) (s1', s2') r ->
       exists (r1: v1).
         t1.step i s1 s1' r1 /\
-        t2.step (extend i r1) s2 s2' r)
+        t2.step (extend i r1) s2 s2' r);
+    chck = app_checks (map_checks fst t1.chck) (map_checks snd t2.chck);
   }
+
+// TODO UNIMPLEMENTED
+let system_contract_instance (#input #input_b #input_ab #state1 #state2 #state3 #a #b: Type)
+  (extend_a: input -> b -> input_b)
+  (extend_ab: input -> a -> b -> input_ab)
+  (assm: system input_b  state1 prop)
+  (guar: system input_ab state2 prop)
+  (arg:  system input    state3 b):
+       system input (state1 & state2 & state3) a =
+  { init = (fun (s1, s2, s3) -> assm.init s1 /\ guar.init s2 /\ arg.init s3);
+    step = (fun i (s1, s2, s3) (s1', s2', s3') r ->
+      exists (rb: b). True);
+    chck = [];
+  }
+
+
+let system_bool_holds (#input #state: Type) (t: system input state bool):
+  system input state prop =
+  system_map (fun b -> prop_holds (b == true)) t
