src/Example.Manual.Antilock.fst
@@ -1,0 +1,184 @@
+module Example.Manual.Antilock
+
+open FStar.Mul
+open FStar.Ref
+
+(* Distance in millimetres, because the wheel is 235mm *)
+type distance = int
+
+(* Represent speed as millimetres per second so we don't need floats.
+   1km/h ~ 277mm/s
+   50km/h ~ 13888mm/s
+*)
+type speed = int
+
+(* millimetres per second per second *)
+type accel = int
+
+(* angular velocity in 1000ths of a revolution per second *)
+type angular_velocity = int
+
+let within_tolerance (b1 b2: int) (tolerance: int): bool =
+  let diff = b1 - b2 in
+  -tolerance <= diff && diff <= tolerance
+
+let wheel_circ: distance = 235 * 2
+
+let gravity: accel = 9800
+
+(* accelerometer tolerance is ±80mg (milligravities?) *)
+let accelerometer_tolerance: speed = gravity * 80 / 1000
+
+let max x y = if x >= y then x else y
+
+(* allow for 5% difference in wheel circumferences.
+  this is about 23mm (almost an inch), at 40 rps ~ 35km/h is 1km/h tolerance. *)
+let wheel_tolerance: angular_velocity = 1000 * 5 / 100 * 40
+let wheel_tolerance_speed: speed = (wheel_tolerance * wheel_circ) / 1000
+
+(* Imperative implementation *)
+
+type inputs = {
+  wheel_front:  angular_velocity;
+  wheel_rear:   angular_velocity;
+  accel_z:      accel;
+}
+type estimate = {
+  speed_lo: speed; speed_hi: speed;
+}
+
+let estimate_init: estimate = {
+  speed_lo = 0; speed_hi = 0;
+}
+
+let estimate_update (i: inputs) (pre: estimate): estimate =
+  let front: speed = (i.wheel_front * wheel_circ) / 1000 in
+  let rear:  speed = (i.wheel_rear  * wheel_circ) / 1000 in
+  let min_vel: speed = min front rear                    in
+  let max_vel: speed = max front rear                    in
+
+  let ok = within_tolerance i.wheel_front i.wheel_rear wheel_tolerance in
+
+  let lo = if ok then min_vel else pre.speed_lo + i.accel_z - accelerometer_tolerance in
+  let hi = if ok then max_vel else pre.speed_hi + i.accel_z + accelerometer_tolerance in
+
+  { speed_lo = lo; speed_hi = hi; }
+
+let estimate_update_accurate (i: inputs) (pre: estimate):
+  Lemma
+    (requires within_tolerance i.wheel_front i.wheel_rear wheel_tolerance)
+    (ensures
+        (let e' = estimate_update i pre in
+        within_tolerance e'.speed_lo e'.speed_hi wheel_tolerance_speed)) =
+  ()
+
+let estimate_update_accuracy_degrades (i: inputs) (pre: estimate) (tol: speed):
+  Lemma
+    (requires within_tolerance pre.speed_lo pre.speed_hi tol)
+    (ensures
+        (let e' = estimate_update i pre in
+        within_tolerance e'.speed_lo e'.speed_hi (tol + accelerometer_tolerance * 2))) =
+  ()
+
+
+module Exp = Pipit.Exp.Base
+module Sugar = Pipit.SugarX4
+
+let previously (e: Sugar.s bool): Sugar.s bool =
+  let open Sugar in
+  rec' (fun p -> fby false p \/ e)
+
+let count_when_previously (e: Sugar.s bool): Sugar.s int =
+  let open Sugar in
+  rec' (fun count ->
+    let prev = fby 0 count in
+    if_then_else e z0 (prev +^ z1)
+  )
+
+let previously_n (n: nat) (e: Sugar.s bool): Sugar.s bool =
+  let open Sugar in
+  previously e /\ count_when_previously e <=^ z n
+
+let veh_speed_estimate (i: Sugar.s inputs): Sugar.s estimate =
+  let open Sugar in
+  let wheel_front = (fun i -> i.wheel_front) <$> i    in
+  let wheel_rear  = (fun i -> i.wheel_rear)  <$> i    in
+  let accel_z     = (fun i -> i.accel_z)     <$> i    in
+  let wheel_circ  = pure wheel_circ                in
+  let z1000       = pure 1000                      in
+  let accelerometer_tolerance = pure accelerometer_tolerance in
+  let mk_estimate lo hi = (fun lo hi -> { speed_lo = lo; speed_hi = hi }) <$> lo <*> hi in
+
+  let front = (wheel_front *^ wheel_circ) /^ z1000 in
+  let rear  = (wheel_rear  *^ wheel_circ) /^ z1000 in
+  let min_vel = min <$> front <*> rear             in
+  let max_vel = max <$> front <*> rear             in
+
+  let ok    = within_tolerance <$> wheel_front <*> wheel_rear <*> pure wheel_tolerance in
+
+  let lo = rec' (fun lo ->
+    if_then_else ok min_vel ((min_vel --> pre lo) +^ accel_z -^ accelerometer_tolerance)) in
+  let hi = rec' (fun hi ->
+    if_then_else ok max_vel ((max_vel --> pre hi) +^ accel_z +^ accelerometer_tolerance)) in
+
+  let est = mk_estimate lo hi in
+
+  check' "veh_speed_estimate_accurate"
+    ((within_tolerance <$> wheel_front <*> wheel_rear <*> pure wheel_tolerance) =>
+     (within_tolerance <$> lo <*> hi <*> pure wheel_tolerance_speed)) (
+  est)
+
+open Pipit.System.Base
+open Pipit.System.Exp
+open Pipit.System.Ind
+open Pipit.System.Det
+module T = FStar.Tactics
+
+// let veh_speed_estimate': system
+
+let run (e: Sugar.s 'a) : Exp.exp [] 'a =
+  let (a, _) = e { fresh = 0 } in
+  a
+
+let sys =
+  system_of_exp (run (veh_speed_estimate (Sugar.m_pure (Exp.XVar (Pipit.Context.Var 100)))))
+
+
+// let prove (fv: sem_freevars): Lemma (ensures base_case (sys fv)) =
+//   assert (base_case (sys fv)) by (T.norm [primops; iota; delta; zeta; nbe]; T.dump "")
+
+let dsys': dsystem inputs (bool & speed & speed & prop) estimate =
+  {
+    init = (true, 0, 0, True);
+    step = (fun i (init, lo, hi, chk_accurate) ->
+        let front = i.wheel_front * wheel_circ / 1000 in
+        let rear  = i.wheel_rear  * wheel_circ / 1000 in
+        let min_vel = min front rear                    in
+        let max_vel = max front rear                    in
+
+        let ok    = within_tolerance i.wheel_front i.wheel_rear wheel_tolerance in
+
+        let lo' =
+            if ok
+            then min_vel
+            else ((if init then min_vel else lo) + i.accel_z - accelerometer_tolerance)
+        in
+        let hi' =
+            if ok
+            then min_vel
+            else ((if init then min_vel else hi) + i.accel_z + accelerometer_tolerance)
+        in
+        let chk_accurate': prop =
+          ok ==> within_tolerance lo' hi' wheel_tolerance_speed
+        in
+        ((false, lo', hi', chk_accurate'),
+          { speed_lo = lo'; speed_hi = hi' })
+      );
+    chck = [("chk_accurate", (fun (_, _, _, c) -> c))];
+  }
+
+let sys' = system_of_dsystem dsys'
+
+let prove (): Lemma (ensures induct1 sys') =
+  assert (base_case sys') by (T.norm [primops; iota; delta; zeta; nbe]; T.dump "");
+  assert (step_case sys') by (T.norm [primops; iota; delta; zeta; nbe]; T.dump "")
