src/Pipit.Exp.Base.fst
@@ -26,6 +26,7 @@ type exp (c: C.context) 'a =
   // Proof terms
   // Contracts for hiding implementation:
   //   (λx. { assumes } body { λr. guarantees })(arg)
+  // TODO: assumes and guarantees should probably be in context c, so they can be CSEd with the main expression. body should be separate to allow separate codegen
   | XContract:
            (assumes: exp ['b] xprop) ->
            (guarantees: exp ['a; 'b] xprop) ->
